src/Dafny/examples/fs/indirect_fs.dfy
@@ -1,4 +1,5 @@
 include "fs.dfy"
+include "ind_block.dfy"
 
 module IndFs
 {
@@ -8,54 +9,8 @@ module IndFs
   import opened JrnlSpec
   import opened Fs
   import opened Marshal
+  import opened IndBlocks
   import C = Collections
-
-  predicate block_has_blknos(b: Block, blknos: seq<Blkno>)
-  {
-    && is_block(b)
-    && b == seq_enc_uint64(blknos)
-    && |blknos| == 512
-  }
-
-  // there are two redundant length expressions in block_has_blknos, we can use
-  // either of them to prove block_has_blknos
-  lemma block_has_blknos_len(b: Block, blknos: seq<Blkno>)
-    requires b == seq_enc_uint64(blknos)
-    requires is_block(b) || |blknos| == 512
-    ensures block_has_blknos(b, blknos)
-  {
-    enc_uint64_len(blknos);
-    assert 4096 == 512*8;
-  }
-
-  lemma zero_block_blknos()
-    ensures block_has_blknos(block0, C.repeat(0 as Blkno, 512))
-  {
-    zero_encode_seq_uint64(512);
-  }
-
-  method encode_blknos(blknos: seq<Blkno>) returns (bs: Bytes)
-    requires |blknos| == 512
-    ensures fresh(bs)
-    ensures block_has_blknos(bs.data, blknos)
-  {
-    var enc := new Encoder(4096);
-    enc.PutInts(blknos);
-    assert enc.enc == C.seq_fmap(encUInt64, blknos);
-    enc.is_complete();
-    bs := enc.Finish();
-    return;
-  }
-
-  method decode_blknos(bs: Bytes, ghost blknos: seq<Blkno>) returns (blknos': seq<Blkno>)
-    requires block_has_blknos(bs.data, blknos)
-    ensures blknos' == blknos
-  {
-    var dec := new Decoder.Init(bs, C.seq_fmap(encUInt64, blknos));
-    assert dec.enc[..512] == dec.enc;
-    blknos' := dec.GetInts(512, blknos);
-    return;
-  }
 
   datatype Idx = direct(k: nat) | indirect(k: nat, m: nat)
   {
