src/Dafny/examples/fs/ind_block.dfy
@@ -1,0 +1,60 @@
+include "../../machine/machine.s.dfy"
+include "../../jrnl/jrnl.s.dfy"
+include "../../util/marshal.i.dfy"
+
+module IndBlocks
+{
+  import opened Machine
+  import opened JrnlSpec
+
+  import opened ByteSlice
+  import opened Marshal
+
+  predicate block_has_blknos(b: Block, blknos: seq<Blkno>)
+  {
+    && is_block(b)
+    && b == seq_enc_uint64(blknos)
+    && |blknos| == 512
+  }
+
+  // there are two redundant length expressions in block_has_blknos, we can use
+  // either of them to prove block_has_blknos
+  lemma block_has_blknos_len(b: Block, blknos: seq<Blkno>)
+    requires b == seq_enc_uint64(blknos)
+    requires is_block(b) || |blknos| == 512
+    ensures block_has_blknos(b, blknos)
+  {
+    enc_uint64_len(blknos);
+    assert 4096 == 512*8;
+  }
+
+  lemma zero_block_blknos()
+    ensures block_has_blknos(block0, C.repeat(0 as Blkno, 512))
+  {
+    zero_encode_seq_uint64(512);
+  }
+
+  method encode_blknos(blknos: seq<Blkno>) returns (bs: Bytes)
+    requires |blknos| == 512
+    ensures fresh(bs)
+    ensures block_has_blknos(bs.data, blknos)
+  {
+    var enc := new Encoder(4096);
+    enc.PutInts(blknos);
+    assert enc.enc == C.seq_fmap(encUInt64, blknos);
+    enc.is_complete();
+    bs := enc.Finish();
+    return;
+  }
+
+  method decode_blknos(bs: Bytes, ghost blknos: seq<Blkno>) returns (blknos': seq<Blkno>)
+    requires block_has_blknos(bs.data, blknos)
+    ensures blknos' == blknos
+  {
+    var dec := new Decoder.Init(bs, C.seq_fmap(encUInt64, blknos));
+    assert dec.enc[..512] == dec.enc;
+    blknos' := dec.GetInts(512, blknos);
+    return;
+  }
+
+}
